thys/ISAT_Basic.thy
@@ -1,0 +1,89 @@
+theory ISAT_Basic
+imports SAT_Basic
+begin
+
+  definition "consistent L \<equiv> \<forall>l\<in>L. neg_lit l\<notin>L"
+
+  definition "set_lits F L \<equiv> { C - neg_lit`L | C. C\<in>F \<and> L \<inter> C = {} }"
+  
+  lemma set_lits_singleton: "set_lits F {l} = set_lit F l"
+    unfolding set_lits_def set_lit_def 
+    by clarsimp
+  
+  
+  lemma set_lits_empty[simp]: "set_lits F {} = F"
+    unfolding set_lits_def by auto
+
+  lemma set_lits_insert': "consistent (insert l L) \<Longrightarrow> set_lits F (insert l L) = (set_lits (set_lit F l) L)"
+    unfolding set_lits_def set_lit_def 
+    apply safe
+    apply clarsimp
+    apply (metis Diff_insert2 Int_Diff empty_Diff)
+    apply clarsimp
+    subgoal for C
+      by (metis Diff_insert2 consistent_def disjoint_insert(2) insertCI insert_Diff_single)
+    done          
+      
+  lemma set_lits_insert[simp]: "consistent (insert l L) \<Longrightarrow> set_lits F (insert l L) = (set_lit (set_lits F L) l)"
+    unfolding set_lits_def set_lit_def 
+    apply (safe; clarsimp)
+    subgoal by (metis DiffD1 Diff_insert)
+    subgoal by blast
+    by (simp add: consistent_def)
+  
+    
+  lemma set_lit_swap: "l1\<noteq>neg_lit l2 \<Longrightarrow> set_lit (set_lit F l1) l2 = set_lit (set_lit F l2) l1"
+    by (smt (verit) consistent_def insert_iff neg_lit_neq(1) neg_neg_lit set_lits_insert set_lits_insert' set_lits_singleton singletonD)
+
+
+  datatype 'l IItem = 
+      I "'l clause" 
+    | Q "'l literal set" 
+    | A_SAT "'l literal set" (* Formula mod model must be sat *)
+    | A_UNSAT "'l literal set" (* Subset of query, and makes formula unsat already *)
+
+
+  type_synonym 'l IState = "'l cnf * 'l literal set option"
+
+
+
+  inductive isat_step where
+    "isat_step (F,q) (I C) (insert C F,q)"
+  | "consistent ls \<Longrightarrow> isat_step (F,None) (Q ls) (F, Some ls)"
+  | "consistent (ls\<union>qls) \<Longrightarrow> sat (set_lits F (ls \<union> qls)) \<Longrightarrow> isat_step (F,Some qls) (A_SAT ls) (F,None)"
+  | "\<lbrakk>consistent ls; ls\<subseteq>qls; \<not>sat(set_lits F ls)\<rbrakk> \<Longrightarrow> isat_step (F,Some qls) (A_UNSAT ls) (F,None)"
+
+
+  fun isat_stepf where
+    "isat_stepf (I C) (F,q) = Some (insert C F, q)"
+  | "isat_stepf (Q ls) (F,None) = (if consistent ls then Some (F,Some ls) else None)"  
+  | "isat_stepf (A_SAT ls) (F,Some qls) = (if consistent (ls\<union>qls) \<and> sat (set_lits F (ls \<union> qls)) then Some (F,None) else None)"
+  | "isat_stepf (A_UNSAT ls) (F,Some qls) = (if consistent ls \<and> ls\<subseteq>qls \<and> \<not>sat(set_lits F ls) then Some (F,None) else None)"
+  | "isat_stepf _ _ = None"
+  
+  lemma "isat_step s l s' \<longleftrightarrow> isat_stepf s l = Some s'"
+    apply (cases "(s,l)" rule: isat_stepf.cases)
+    by (auto simp: isat_step.simps)
+  
+  
+  find_consts "_ option" name: fold
+  
+  fun fold_option where
+    "fold_option f [] s = Some s"
+  | "fold_option f (x#xs) s = (Option.bind (f x s) (fold_option f xs))"
+
+  definition "ISound iis \<equiv> fold_option isat_stepf iis ({},None)"
+    
+  xxx, next step: formalize checker LTS, with read actions from interaction protocol and proof. (see paper)
+  
+  
+  oops  xxx: phrase that as mfold over option monad!
+  
+  
+  
+  
+  
+  
+  
+
+end
